examples/ghc/module-edits/CoreSubst/midamble.v
@@ -1,3 +1,6 @@
+Require Import Id.
+Require Import Core.
+
 Instance Default_Subst : GHC.Err.Default Subst :=
   GHC.Err.Build_Default _ (Mk_Subst GHC.Err.default GHC.Err.default tt tt).
 
